io/IIO.Behavior.fst
@@ -1,0 +1,38 @@
+module IIO.Behavior
+
+open FStar.Ghost
+open FStar.FunctionalExtensionality
+
+open BeyondCriteria
+open IIO
+
+assume val __reify_IIOwp (#a:Type) (#wp:Hist.hist a) (#fl:tflag) ($f:unit -> IIOwp a fl wp) : GTot (dm_giio a fl wp)
+
+(* We define `beh` that returns the set of traces produced by a whole program.
+   Since whole programs start with the empty trace, 
+   the local trace contains the complete trace.
+
+   `theta` is a weakest precondtion monad, and we need it to be
+   a post-condition. Looking at Kenji's thesis, we can apply the
+   'backward predicate transformer 2.3.4' and the 
+   'pre-/postcondition transformer 2.3.2' to obtain
+   the 'set' of traces produces by the whole program. *)
+val beh_giio : (list string -> GTot (dm_giio int AllActions trivial_hist)) -> trace_property #event
+let beh_giio ws tr =
+  match tr with
+  | Infinite_trace _ _ -> False
+  | Finite_trace args lt res -> 
+   (* We verify specs of whole programs, thus, instead of having
+      properties forall histories, we can specialize it for the
+      empty history *)
+    forall p. dm_giio_theta (ws args) p [] ==> p lt res
+
+val _beh : (list string -> IIO int AllActions (fun _ -> True) (fun _ _ _ -> True)) -> trace_property #event
+let _beh ws =
+  beh_giio (fun args -> 
+    let ws' : unit -> IIO int AllActions (fun _ -> True) (fun _ _ _ -> True) = (fun () -> ws args) in
+    __reify_IIOwp (fun () -> ws args))
+
+irreducible
+val beh : (list string -> IIO int AllActions (fun _ -> True) (fun _ _ _ -> True)) ^-> trace_property #event
+let beh = on_domain _ (fun ws -> _beh ws)
